Finished progress (up to change-of-modality operators).

coq/Corps/Beta.v
@@ -10,10 +10,39 @@ Section BetaReduction.
   #[local] Notation mod := (mod PName).
   Context {CanSend CanUp CanDown : mod -> mod -> Prop}.
   #[local] Notation Typed := (@Typed PName CanSend CanUp CanDown).
+  #[local] Notation TypedSubst := (@TypedSubst PName CanSend CanUp CanDown).
+
+  Definition single_subst (v : expr) : substitution :=
+    fun n => match n with
+          | 0 => v
+          | S n' => var n'
+          end.
+
+  Lemma singlesubst_typed : forall (Γ : Ctxt) (v : expr) (τ : type),
+      Typed Γ v τ -> TypedSubst (add_var Γ base τ) (single_subst v) Γ.
+  Proof using.
+    intros Γ v τ typ; split; cbn; [reflexivity| intros x m eq].
+    destruct x; cbn in *; subst.
+    - apply type_ext with (Γ := Γ); [exact typ | apply add_base_lock].
+    - apply @VarTyping with (m := mod_app m (locks Γ x)); cbn; [|reflexivity].
+      rewrite eq; apply surjective_pairing.
+  Qed.
 
   (* substitute v for the variable 0 in e *)
-  Definition singlesubst (e v : expr) :=
-    subst e (fun n => match n with | 0 => v |S n' => var n' end).
+  Definition subst1 (e v : expr) :=
+    subst e (single_subst v).
+
+  Lemma subst1_typed : forall Γ e v τ1 τ2,
+      Typed (add_var Γ base τ1) e τ2 ->
+      Typed Γ v τ1 ->
+      Typed Γ (subst1 e v) τ2.
+  Proof using.
+    intros Γ e v τ1 τ2 typed_e typed_v; 
+      unfold subst1; apply subst_typed with (Γ := add_var Γ base τ1);
+      [ exact typed_e
+      | apply singlesubst_typed; exact typed_v
+      ].
+  Qed.
 
   Inductive stepβ : expr -> expr -> Prop :=
     stepAt (p : PName) {e1 e2 : expr} (step : stepβ e1 e2) : stepβ (atE p e1) (atE p e2)
@@ -21,8 +50,8 @@ Section BetaReduction.
     : stepβ (letAt p e11 e2) (letAt p e12 e2)
   | stepLet2 (p : PName) (e1 : expr) {e21 e22 : expr} (step : stepβ e21 e22)
     : stepβ (letAt p e1 e21) (letAt p e1 e22)
-  (* | stepLetβ (p : PName) (e1 e2 : expr) : *)
-  (*   stepβ (letAt p (atE p e1) e2) (* Unclear what to do here! *) *)
+  | stepLetβ (p : PName) (e1 e2 : expr) :
+    stepβ (letAt p (atE p e1) e2) (subst1 e2 e1)
   | stepPair1 {e11 e12 : expr} (step : stepβ e11 e12) (e2 : expr) : stepβ (pair e11 e2) (pair e12 e2)
   | stepPair2 (e1 : expr) {e21 e22 : expr} (step : stepβ e21 e22) : stepβ (pair e1 e21) (pair e1 e22)
   | stepPi1 {e1 e2 : expr} (step : stepβ e1 e2) : stepβ (pi1 e1) (pi1 e2)
@@ -37,16 +66,15 @@ Section BetaReduction.
     : stepβ (caseE e1 e21 e3) (caseE e1 e22 e3)
   | stepCaseE3 (e1 e2 : expr) {e31 e32 : expr} (step : stepβ e31 e32)
     : stepβ (caseE e1 e2 e31) (caseE e1 e2 e32)
-  | stepCaseInl (e1 e2 e3 : expr) : stepβ (caseE (inl e1) e2 e3) (singlesubst e3 e1)
-  (* Do I really want stepEfqlInner? *)
+  | stepCaseInl (e1 e2 e3 : expr) : stepβ (caseE (inl e1) e2 e3) (subst1 e2 e1)
+  | stepCaseInr (e1 e2 e3 : expr) : stepβ (caseE (inr e1) e2 e3) (subst1 e3 e1)
   | stepEfqlInner {e1 e2 : expr} (step : stepβ e1 e2) : stepβ (efql e1) (efql e2)
-  (* | stepEfql (e1 e2 : expr) : stepβ (efql e1) e2 (* Should e2 have to be in normal form? *) *)
   | stepLam (t : type) {e1 e2 : expr} (step : stepβ e1 e2) : stepβ (lam t e1) (lam t e2)
   | stepApp1 {e11 e12 : expr} (step : stepβ e11 e12) (e2 : expr)
     : stepβ (appE e11 e2) (appE e12 e2)
   | stepApp2 (e1 : expr) {e21 e22 : expr} (step : stepβ e21 e22)
     : stepβ (appE e1 e21) (appE e1 e22)
-  | stepAppLam (t : type) (e1 e2 : expr) : stepβ (appE (lam t e1) e2) (singlesubst e1 e2).
+  | stepAppLam (t : type) (e1 e2 : expr) : stepβ (appE (lam t e1) e2) (subst1 e1 e2).
 
   
   Theorem preservation : forall e1 e2 Γ τ, Typed Γ e1 τ -> stepβ e1 e2 -> Typed Γ e2 τ.
@@ -60,9 +88,17 @@ Section BetaReduction.
                end
            end;
       try (econstructor; eauto; fail); try (inversion typ; subst; assumption).
-    - admit.
-    - admit.
-  Admitted.
-
+    - inversion typ1; subst.
+      unfold subst1.
+      apply subst_typed with (Γ := add_var Γ (Types.ptm p) τ); auto.
+      split; cbn; [reflexivity|].
+      intros x m; destruct x; cbn; intro eq; subst; auto.
+      apply @VarTyping with (m := mod_app m (locks Γ x)); cbn.
+      rewrite eq; apply surjective_pairing.
+      reflexivity.
+    - inversion typ1; subst; eapply subst1_typed; eauto.
+    - inversion typ1; subst; eapply subst1_typed; eauto.
+    - inversion typ1; subst; eapply subst1_typed; eauto.
+  Qed.
 
 End BetaReduction.
